Cook_Levin_IMP/IMP-_To_SAS+/IMP-_To_SAS+_HOL/IMP-_To_IMP--/IMP_Minus_To_IMP_Minus_Minus.thy
@@ -10,25 +10,25 @@ begin
 text \<open> We give a reduction from IMP- to IMP--. The reduction works by bit blasting each register
        of IMP- into several registers in IMP-- each holding a single bit. Arithmetic operations
        and assignment in IMP- are replaced by the binary operations defined in the Binary Operations
-       theory. For WHILE and IF, we replace the condition of a single register's content being 
+       theory. For WHILE and IF, we replace the condition of a single register's content being
        non-zero by checking whether any of the bits in the translated state is non-zero. \<close>
 
 definition var_bit_list:: "nat \<Rightarrow> vname \<Rightarrow> vname list" where
 "var_bit_list n v = map (\<lambda>i. var_bit_to_var (v, i)) [0..<n]"
 
 lemma exists_non_zero_in_var_bit_list_iff:
-  assumes "finite (range s)" "Max (range s) < 2 ^ n" 
+  assumes "finite (range s)" "Max (range s) < 2 ^ n"
   shows "(\<exists>b\<in>set (var_bit_list n v). IMP_Minus_State_To_IMP_Minus_Minus s n b \<noteq> Some Zero)
-      \<longleftrightarrow> s v > 0" 
-  using assms 
-  by(auto simp: var_bit_list_def IMP_Minus_State_To_IMP_Minus_Minus_def 
+      \<longleftrightarrow> s v > 0"
+  using assms
+  by(auto simp: var_bit_list_def IMP_Minus_State_To_IMP_Minus_Minus_def
       IMP_Minus_State_To_IMP_Minus_Minus_with_operands_a_b_def has_bit_one_then_greater_zero
       greater_zero_then_has_bit_one)
 
 fun IMP_Minus_To_IMP_Minus_Minus:: "IMP_Minus_com \<Rightarrow> nat \<Rightarrow> IMP_Minus_Minus_com" where
 "IMP_Minus_To_IMP_Minus_Minus Com.SKIP n = SKIP" |
 "IMP_Minus_To_IMP_Minus_Minus (Com.Assign v aexp) n = assignment_to_binary n v aexp" |
-"IMP_Minus_To_IMP_Minus_Minus (Com.Seq c1 c2) n = 
+"IMP_Minus_To_IMP_Minus_Minus (Com.Seq c1 c2) n =
   (IMP_Minus_To_IMP_Minus_Minus c1 n ;; IMP_Minus_To_IMP_Minus_Minus c2 n )" |
 "IMP_Minus_To_IMP_Minus_Minus (Com.If v c1 c2) n = (IF (var_bit_list n v)\<noteq>0 THEN
   IMP_Minus_To_IMP_Minus_Minus c1 n ELSE IMP_Minus_To_IMP_Minus_Minus c2 n)" |
@@ -41,7 +41,7 @@ lemma finite_range_stays_finite: "(c1, s1) \<Rightarrow>\<^bsup>t\<^esup> s2 \<L
   apply auto
   by (metis Un_infinite image_Un sup_top_right)
 
-lemma Max_insert_le_when: 
+lemma Max_insert_le_when:
   "\<lbrakk>finite (range (s :: vname \<Rightarrow> nat)); y < r;  Max (range s) < r\<rbrakk> \<Longrightarrow> Max (range (s(x := y))) < r"
 proof(goal_cases)
   case 1
@@ -61,21 +61,21 @@ proof(goal_cases)
     by simp
 qed
 
-lemma IMP_Minus_space_growth: 
+lemma IMP_Minus_space_growth:
   "\<lbrakk>(c1, s1) \<Rightarrow>\<^bsup>t\<^esup> s2; finite (range s1);
-    max (Max (range s1)) (Max_Constant.max_constant c1) < 2 ^ k\<rbrakk> \<Longrightarrow> 
+    max (Max (range s1)) (Max_Constant.max_constant c1) < 2 ^ k\<rbrakk> \<Longrightarrow>
     (finite (range s2) \<and> Max (range s2) < (2 :: nat) ^ (k + t))"
 proof(induction c1 s1 t s2 arbitrary: k rule: big_step_t_induct)
   case (Skip s)
-  thus ?case 
-  by (smt add_lessD1 le_less_trans le_simps max_def mult_2 mult_Suc_right not_le plus_1_eq_Suc 
+  thus ?case
+  by (smt add_lessD1 le_less_trans le_simps max_def mult_2 mult_Suc_right not_le plus_1_eq_Suc
       power.simps power.simps power_add)
 next
   case (Assign x a s)
   hence "AExp.aval a s < 2 * 2 ^ k"
-    by (auto intro!: aval_le_when) 
+    by (auto intro!: aval_le_when)
   hence "Max (range (s(x := aval a s))) < 2 ^ (k + Suc (Suc 0))"
-    using Assign 
+    using Assign
     by (fastforce simp: eval_nat_numeral intro!: trans_less_add2 Max_insert_le_when)
   thus ?case using Assign
     using finite_range_stays_finite
@@ -83,7 +83,7 @@ next
 next
   case (Seq c1 s1 x s2 c2 y s3 z)
   hence "finite (range s2)"
-    using finite_range_stays_finite 
+    using finite_range_stays_finite
     by blast
   hence "s2 a < 2 ^ (k + x)" for a
     using Seq \<open>finite (range s1)\<close> \<open>finite (range s2)\<close>
@@ -92,43 +92,43 @@ next
     using Seq
     by simp
   hence "max_constant c2 < (2 :: nat) ^ (k + x)"
-    using bigstep_progress Seq 
+    using bigstep_progress Seq
     by (auto simp: eval_nat_numeral intro: le_less_trans less_imp_le_nat  n_less_n_mult_m)
   hence "s3 a < (2 :: nat) ^ (k + x + y)" for a using Seq \<open>finite (range s2)\<close>
     by fastforce
   moreover have "finite (range s3)"
-    using Seq.hyps(2) \<open>finite (range s2)\<close> finite_range_stays_finite 
+    using Seq.hyps(2) \<open>finite (range s2)\<close> finite_range_stays_finite
     by blast
   ultimately show ?case using Seq
     by (auto simp: add.assoc eval_nat_numeral)
 next
   case (WhileTrue s1 b c x s2 y s3 z)
   hence "finite (range s2)" using finite_range_stays_finite by blast
-  hence "s2 a < 2 ^ (k + x)" for a 
+  hence "s2 a < 2 ^ (k + x)" for a
     using WhileTrue \<open>finite (range s1)\<close> \<open>finite (range s2)\<close>
     by auto
   have "max_constant (WHILE b\<noteq>0 DO c)  < 2 ^ k"
     using WhileTrue
     by simp
   hence "max_constant (WHILE b\<noteq>0 DO c) < (2 :: nat) ^ (k + x)"
-    by (metis One_nat_def WhileTrue.hyps(2) bigstep_progress le_less_trans lessI 
-        less_add_same_cancel1 less_imp_le_nat numeral_2_eq_2 power_strict_increasing_iff) 
+    by (metis One_nat_def WhileTrue.hyps(2) bigstep_progress le_less_trans lessI
+        less_add_same_cancel1 less_imp_le_nat numeral_2_eq_2 power_strict_increasing_iff)
   hence "\<forall>a. s3 a < (2 :: nat) ^ (k + x + y)"
-    using WhileTrue \<open>finite (range s2)\<close> 
+    using WhileTrue \<open>finite (range s2)\<close>
     by fastforce
   moreover have "finite (range s3)"
-    using WhileTrue.hyps(3) \<open>finite (range s2)\<close> finite_range_stays_finite 
+    using WhileTrue.hyps(3) \<open>finite (range s2)\<close> finite_range_stays_finite
     by blast
-  ultimately show ?case using WhileTrue 
+  ultimately show ?case using WhileTrue
     by (auto simp: group_cancel.add1 mult_2 trans_less_add2)
-qed (auto simp: numeral_2_eq_2 trans_less_add1) 
+qed (auto simp: numeral_2_eq_2 trans_less_add1)
 
-lemma power_of_two_minus: "2 ^ a * c < 2 ^ b \<Longrightarrow> c < (2 :: nat) ^ (b - a)" 
+lemma power_of_two_minus: "2 ^ a * c < 2 ^ b \<Longrightarrow> c < (2 :: nat) ^ (b - a)"
 proof(induction a arbitrary: c)
   case (Suc a)
   hence "2 * c < 2 ^ (b - a)" by auto
   thus ?case
-    by (metis One_nat_def Suc_diff_Suc bot_nat_0.not_eq_extremum less_Suc0 
+    by (metis One_nat_def Suc_diff_Suc bot_nat_0.not_eq_extremum less_Suc0
               nat_mult_less_cancel_disj numeral_2_eq_2 power_0 power_Suc zero_less_diff zero_less_power)
 qed auto
 
@@ -136,26 +136,26 @@ lemma power_of_two_increase_exponent_le: "(2 :: nat) ^ (a + b) * c < r \<Longrig
   by(auto intro: dual_order.strict_trans2)
 
 lemma move_exponent_to_rhs: "c < (2 :: nat) ^ (a - b) \<Longrightarrow> 2 ^ b * c < 2 ^ a"
-  by (smt One_nat_def diff_mult_distrib2 gr_zeroI less_Suc0 
-      linordered_semidom_class.add_diff_inverse mult_eq_0_iff order.asym power.simps(1) 
+  by (smt One_nat_def diff_mult_distrib2 gr_zeroI less_Suc0
+      linordered_semidom_class.add_diff_inverse mult_eq_0_iff order.asym power.simps(1)
       power_add power_eq_0_iff zero_less_diff zero_neq_numeral)
 
 subsection \<open>Correctness\<close>
 
-text \<open>First direction of the correctness statement. We show that when an IMP- program run from a 
-      state where all values are bounded terminates in some state, then the translated IMP-- program 
-      started on the translated initial state will terminate in the translated final state, after 
-      a number of steps that is polynomially bigger than the number of steps the IMP- program run 
+text \<open>First direction of the correctness statement. We show that when an IMP- program run from a
+      state where all values are bounded terminates in some state, then the translated IMP-- program
+      started on the translated initial state will terminate in the translated final state, after
+      a number of steps that is polynomially bigger than the number of steps the IMP- program run
       for. The constants appearing in the polynomial bound have no significance.  \<close>
 
-lemma IMP_Minus_To_IMP_Minus_Minus: 
-  assumes 
+lemma IMP_Minus_To_IMP_Minus_Minus:
+  assumes
     "(c1 :: IMP_Minus_com, s1) \<Rightarrow>\<^bsup>t\<^esup> s2"
     "finite (range s1)"
-    "n > t" 
+    "n > t"
     "((2 :: nat) ^ t) * (max (Max (range s1)) (max_constant c1)) < 2 ^ n"
   shows
-    "t_small_step_fun (100 * n * (t - 1) + 50) 
+    "t_small_step_fun (100 * n * (t - 1) + 50)
       (IMP_Minus_To_IMP_Minus_Minus c1 n, IMP_Minus_State_To_IMP_Minus_Minus s1 n)
      = (SKIP, IMP_Minus_State_To_IMP_Minus_Minus s2 n)"
   using assms
@@ -166,7 +166,7 @@ proof(induction c1 s1 t s2 rule: big_step_t_induct)
   ultimately show ?case
     apply(subst t_small_step_fun_increase_time[where ?t="50 * (n + 1)"])
     by (auto simp: aval_le_when IMP_Minus_State_To_IMP_Minus_Minus_def fun_eq_iff
-             intro!: assignment_to_binary_correct[simplified] 
+             intro!: assignment_to_binary_correct[simplified]
              split!: option.splits)
 next
   case (Seq c1 s1 x s2 c2 y s3 z)
@@ -176,19 +176,19 @@ next
     by (meson leD leI less_le_trans mult_less_cancel2)
   hence "2 ^ x * max (Max (range s1)) (max_constant c1) < 2 ^ n"
     by (simp add: nat_mult_max_right)
-  have "max (Max (range s1)) (max_constant (c1)) < 2 ^ (n - z)" 
-    using power_of_two_minus Seq.prems(3) 
+  have "max (Max (range s1)) (max_constant (c1)) < 2 ^ (n - z)"
+    using power_of_two_minus Seq.prems(3)
     by fastforce
-  have "Max (range s2) < 2 ^ (n - y)" 
-    using 
-      IMP_Minus_space_growth[OF \<open>(c1, s1) \<Rightarrow>\<^bsup> x \<^esup> s2\<close> \<open>finite (range s1)\<close> 
+  have "Max (range s2) < 2 ^ (n - y)"
+    using
+      IMP_Minus_space_growth[OF \<open>(c1, s1) \<Rightarrow>\<^bsup> x \<^esup> s2\<close> \<open>finite (range s1)\<close>
                                 \<open>max (Max (range s1)) (max_constant (c1)) < 2 ^ (n - z)\<close>]
       \<open>z = x + y\<close> \<open>n > z \<close>
     by auto
   hence "2 ^ y * Max (range s2) < 2 ^ n"
     using move_exponent_to_rhs
     by blast
- moreover have "2 ^ y * max_constant c2 < 2 ^ n" 
+ moreover have "2 ^ y * max_constant c2 < 2 ^ n"
     using \<open>z = x + y\<close> \<open>2 ^ z * max (Max (range s1)) (max_constant (c1;; c2)) < 2 ^ n\<close>
           power_of_two_increase_exponent_le[where ?b=x]
     by(auto simp: add.commute nat_mult_max_right)
@@ -196,7 +196,7 @@ next
     by simp
   moreover have "finite (range s2)" using finite_range_stays_finite Seq
     by simp
-  ultimately show ?case using Seq \<open>2 ^ x * max (Max (range s1)) (max_constant c1) < 2 ^ n\<close> 
+  ultimately show ?case using Seq \<open>2 ^ x * max (Max (range s1)) (max_constant c1) < 2 ^ n\<close>
     apply (subst IMP_Minus_To_IMP_Minus_Minus.simps)
     apply(rule seq_terminates_when[where ?t1.0="100 * n * (x - Suc 0) + 50" and
           ?t2.0="100 * n * (y - Suc 0) + 50"])
@@ -207,63 +207,63 @@ next
     by (auto simp: algebra_simps)
 next
   case (IfTrue s b c1 x t y c2)
-  hence "(2 ^ y) * Max (range s) < 2 ^ n" 
+  hence "(2 ^ y) * Max (range s) < 2 ^ n"
     by (meson le_less_trans max.cobounded1 move_exponent_to_rhs power_of_two_minus)
   hence "Max (range s) < 2 ^ n" by(auto intro: le_less_trans[OF _ \<open>2 ^ y * Max (range s) < 2 ^ n\<close>])
-  thus ?case apply(simp only: t_small_step_fun_terminate_iff) 
+  thus ?case apply(simp only: t_small_step_fun_terminate_iff)
     using IfTrue apply(simp add: t_small_step_fun_small_step_fun exists_non_zero_in_var_bit_list_iff)
     apply(rule t_small_step_fun_increase_time[where ?t="100 * n * (x - 1) + 50"])
      apply(cases x)
-      using bigstep_progress IfTrue.IH bigstep_progress 
+      using bigstep_progress IfTrue.IH bigstep_progress
     by(fastforce simp: nat_mult_max_right)+
 next
   case (IfFalse s b c2 x t y c1)
-  hence "(2 ^ y) * Max (range s) < 2 ^ n" 
+  hence "(2 ^ y) * Max (range s) < 2 ^ n"
     by (meson le_less_trans max.cobounded1 move_exponent_to_rhs power_of_two_minus)
   hence "Max (range s) < 2 ^ n" by(auto intro: le_less_trans[OF _ \<open>2 ^ y * Max (range s) < 2 ^ n\<close>])
-  then show ?case            
-    apply(subst t_small_step_fun_terminate_iff) 
+  then show ?case
+    apply(subst t_small_step_fun_terminate_iff)
     using IfFalse
     using t_small_step_fun_small_step_fun exists_non_zero_in_var_bit_list_iff
     apply simp
     apply(rule t_small_step_fun_increase_time[where ?t="100 * n * (x - 1) + 50"])
-     apply(cases x) 
-    using bigstep_progress IfFalse.IH bigstep_progress 
+     apply(cases x)
+    using bigstep_progress IfFalse.IH bigstep_progress
     by(fastforce simp: nat_mult_max_right)+
 next
   case (WhileFalse s b c)
-  hence "(2 ^ Suc (Suc 0)) * Max (range s) < 2 ^ n" 
+  hence "(2 ^ Suc (Suc 0)) * Max (range s) < 2 ^ n"
     by (meson le_less_trans max.cobounded1 move_exponent_to_rhs power_of_two_minus)
-  hence "Max (range s) < 2 ^ n" 
+  hence "Max (range s) < 2 ^ n"
     by(auto intro: le_less_trans[OF _ \<open>(2 ^ Suc (Suc 0)) * Max (range s) < 2 ^ n\<close>])
-  then show ?case using WhileFalse  
-    by(simp add: t_small_step_fun_terminate_iff exists_non_zero_in_var_bit_list_iff)  
+  then show ?case using WhileFalse
+    by(simp add: t_small_step_fun_terminate_iff exists_non_zero_in_var_bit_list_iff)
 next
   case (WhileTrue s1 b c x s2 y s3 z)
-  hence "(2 ^ z) * Max (range s1) < 2 ^ n" 
+  hence "(2 ^ z) * Max (range s1) < 2 ^ n"
     by (meson le_less_trans max.cobounded1 move_exponent_to_rhs power_of_two_minus)
   hence "Max (range s1) < 2 ^ n" by(auto intro: le_less_trans[OF _ \<open>2 ^ z * Max (range s1) < 2 ^ n\<close>])
   have "(2 :: nat) ^ x \<le> 2 ^ z" using WhileTrue by simp
-  hence "((2 :: nat) ^ x) * max (Max (range s1)) (max_constant (WHILE b\<noteq>0 DO c)) < 2 ^ n" 
+  hence "((2 :: nat) ^ x) * max (Max (range s1)) (max_constant (WHILE b\<noteq>0 DO c)) < 2 ^ n"
     using \<open>2 ^ z * max (Max (range s1)) (max_constant (WHILE b\<noteq>0 DO c)) < 2 ^ n\<close>
     by (meson leD leI less_le_trans mult_less_cancel2)
   hence "2 ^ x * max (Max (range s1)) (max_constant c) < 2 ^ n" by (simp add: nat_mult_max_right)
-  have "max (Max (range s1)) (max_constant c) < 2 ^ (n - z)" 
+  have "max (Max (range s1)) (max_constant c) < 2 ^ (n - z)"
     using power_of_two_minus WhileTrue by (metis Max_Constant.max_constant.simps)
-  have "Max (range s2) < 2 ^ (n - (y + 1))" 
-    using IMP_Minus_space_growth[OF \<open>(c, s1) \<Rightarrow>\<^bsup> x \<^esup> s2\<close> \<open>finite (range s1)\<close> 
+  have "Max (range s2) < 2 ^ (n - (y + 1))"
+    using IMP_Minus_space_growth[OF \<open>(c, s1) \<Rightarrow>\<^bsup> x \<^esup> s2\<close> \<open>finite (range s1)\<close>
         \<open>max (Max (range s1)) (max_constant c) < 2 ^ (n - z)\<close>] \<open>1 + x + y = z\<close> \<open>n > z \<close> by auto
   hence "2 ^ (y + 1) * Max (range s2) < 2 ^ n" using move_exponent_to_rhs by blast
-  moreover have "2 ^ (y + 1) * max_constant  (WHILE b\<noteq>0 DO c) < 2 ^ n" 
+  moreover have "2 ^ (y + 1) * max_constant  (WHILE b\<noteq>0 DO c) < 2 ^ n"
     using \<open>1 + x + y = z\<close> \<open>2 ^ z * max (Max (range s1)) (max_constant (WHILE b\<noteq>0 DO c)) < 2 ^ n\<close>
-      power_of_two_increase_exponent_le[where ?a="1 + y" and ?b=x] 
+      power_of_two_increase_exponent_le[where ?a="1 + y" and ?b=x]
     by(auto simp: add.commute nat_mult_max_right)
-  ultimately have "2 ^ (y + 1) * max (Max (range s2)) (max_constant (WHILE b\<noteq>0 DO c)) < 2 ^ n" 
+  ultimately have "2 ^ (y + 1) * max (Max (range s2)) (max_constant (WHILE b\<noteq>0 DO c)) < 2 ^ n"
     by simp
   moreover have "finite (range s2)" using finite_range_stays_finite WhileTrue by simp
-  ultimately show ?case using Seq \<open>2 ^ x * max (Max (range s1)) (max_constant c) < 2 ^ n\<close> 
-    apply(simp only: t_small_step_fun_terminate_iff) 
-    using \<open>s1 b \<noteq> 0\<close> \<open>finite (range s1)\<close> \<open>Max (range s1) < 2 ^ n\<close> 
+  ultimately show ?case using Seq \<open>2 ^ x * max (Max (range s1)) (max_constant c) < 2 ^ n\<close>
+    apply(simp only: t_small_step_fun_terminate_iff)
+    using \<open>s1 b \<noteq> 0\<close> \<open>finite (range s1)\<close> \<open>Max (range s1) < 2 ^ n\<close>
     apply(simp add: exists_non_zero_in_var_bit_list_iff)
     apply(rule seq_terminates_when[where ?t1.0="100 * n * (x - Suc 0) + 50" and
           ?t2.0="100 * n * (y - Suc 0) + 50"])
@@ -277,19 +277,19 @@ text \<open>The other direction. Observe that we assume that the IMP- program te
 
 lemma IMP_Minus_Minus_To_IMP_Minus_aux:
   assumes "(c :: IMP_Minus_com, s1) \<Rightarrow>\<^bsup>t'\<^esup> s2"
-    "t' \<le> t" 
+    "t' \<le> t"
     "finite (range s1)"
-    "n > t" 
+    "n > t"
     "((2 :: nat) ^ t) * (max (Max (range s1)) (max_constant c)) < 2 ^ n"
-    "t_small_step_fun t'' 
+    "t_small_step_fun t''
       (IMP_Minus_To_IMP_Minus_Minus c n, IMP_Minus_State_To_IMP_Minus_Minus s1 n)
      = (SKIP, s2')"
-  shows 
+  shows
     "s2' = IMP_Minus_State_To_IMP_Minus_Minus s2 n"
 proof -
-  have "t_small_step_fun (100 * n * (t' - 1) + 50) 
+  have "t_small_step_fun (100 * n * (t' - 1) + 50)
       (IMP_Minus_To_IMP_Minus_Minus c n, IMP_Minus_State_To_IMP_Minus_Minus s1 n)
-     = (SKIP, IMP_Minus_State_To_IMP_Minus_Minus s2 n)" 
+     = (SKIP, IMP_Minus_State_To_IMP_Minus_Minus s2 n)"
     using assms by(fastforce intro: IMP_Minus_To_IMP_Minus_Minus dual_order.strict_trans2)
   thus ?thesis by(metis Pair_inject assms less_imp_le_nat not_less t_small_step_fun_increase_time)
 qed
@@ -299,49 +299,49 @@ subsection \<open>Variables\<close>
 text \<open>We give a few lemmas that specify what variables appear in translated IMP-- programs. \<close>
 
 lemma IMP_Minus_To_IMP_Minus_Minus_variables:
-  "n > 0 \<Longrightarrow> set (enumerate_variables (IMP_Minus_To_IMP_Minus_Minus c n)) \<subseteq> 
+  "n > 0 \<Longrightarrow> set (enumerate_variables (IMP_Minus_To_IMP_Minus_Minus c n)) \<subseteq>
     { var_bit_to_var (w, i) | w i. i < n \<and> w \<in> set (Max_Constant.all_variables c) }
     \<union> { operand_bit_to_var (op, i) | op i. i < n \<and> (op = CHR ''a'' \<or> op = CHR ''b'') }
-    \<union> { ''carry'' }" 
+    \<union> { ''carry'' }"
 proof(induction c)
   case SKIP
   then show ?case by(auto simp: enumerate_variables_def)
 next
-  case (Assign v a) 
+  case (Assign v a)
   thus ?case using assignment_to_binary_variables[where ?n=n and ?v=v and ?a=a] by auto
 next
   case (Seq c1 c2)
-  then show ?case by(auto simp: set_enumerate_variables_seq) 
+  then show ?case by(auto simp: set_enumerate_variables_seq)
 next
   case (If x1 c1 c2)
-  then show ?case by(auto simp: set_enumerate_variables_if var_bit_list_def) 
+  then show ?case by(auto simp: set_enumerate_variables_if var_bit_list_def)
 next
   case (While x1 c)
-  then show ?case by(auto simp: set_enumerate_variables_while var_bit_list_def) 
+  then show ?case by(auto simp: set_enumerate_variables_while var_bit_list_def)
 qed
 
-lemma card_of_set_comprehension_of_set_list: "card { f x |x. x \<in> set l} \<le> length (remdups l)" 
+lemma card_of_set_comprehension_of_set_list: "card { f x |x. x \<in> set l} \<le> length (remdups l)"
 proof(induction l)
   case (Cons a l)
   have "{ f x |x. x \<in> set (a # l)} = { f a } \<union> { f x |x. x \<in> set l}" by auto
   thus ?case using Cons apply auto
      apply (metis (mono_tags, lifting) card.infinite card_insert_if finite_insert mem_Collect_eq)
-    by (metis (no_types, lifting) Suc_le_mono card.infinite card_insert_disjoint finite_insert 
+    by (metis (no_types, lifting) Suc_le_mono card.infinite card_insert_disjoint finite_insert
         insert_absorb le_SucI)
 qed auto
 
-lemma card_union_le: "card U \<le> a \<Longrightarrow> card W \<le> b \<Longrightarrow> card (U \<union> W) \<le> (a + b)"  
+lemma card_union_le: "card U \<le> a \<Longrightarrow> card W \<le> b \<Longrightarrow> card (U \<union> W) \<le> (a + b)"
   using card_Un_le[where ?A=U and ?B=W] by simp
 
-lemma card_union_le_intro: "card U \<le> a \<Longrightarrow> card W \<le> b \<Longrightarrow> c \<ge> a + b \<Longrightarrow> card (U \<union> W) \<le> c"  
+lemma card_union_le_intro: "card U \<le> a \<Longrightarrow> card W \<le> b \<Longrightarrow> c \<ge> a + b \<Longrightarrow> card (U \<union> W) \<le> c"
   using card_Un_le[where ?A=U and ?B=W] by simp
 
 lemma IMP_Minus_To_IMP_Minus_Minus_variables_length:
   assumes "n > 0"
   shows "length (enumerate_variables (IMP_Minus_To_IMP_Minus_Minus c n)) \<le>
-    (n + 1) * (Max_Constant.num_variables c) + 2 * n + 1" 
-proof - 
-  have "finite { var_bit_to_var (w, i) | w i. i < n \<and> w \<in> set (Max_Constant.all_variables c) } 
+    (n + 1) * (Max_Constant.num_variables c) + 2 * n + 1"
+proof -
+  have "finite { var_bit_to_var (w, i) | w i. i < n \<and> w \<in> set (Max_Constant.all_variables c) }
     \<and> card { var_bit_to_var (w, i) | w i. i < n \<and> w \<in> set (Max_Constant.all_variables c) }
     \<le> n * (Max_Constant.num_variables c)"
   proof(induction n)
@@ -351,7 +351,7 @@ proof -
         \<union> { var_bit_to_var (w, n) |w. w \<in> set (Max_Constant.all_variables c) }"
       by auto
     moreover have "card {var_bit_to_var (w, n) |w. w \<in> set (Max_Constant.all_variables c)}
-      \<le> num_variables c" 
+      \<le> num_variables c"
       using card_of_set_comprehension_of_set_list num_variables_def by fastforce
     ultimately show ?case using Suc by (simp add: card_union_le sup_commute)
   qed auto
@@ -366,7 +366,7 @@ proof -
         \<union> { operand_bit_to_var (CHR ''a'', n), operand_bit_to_var (CHR ''b'', n)}" by auto
     thus ?case using Suc by(auto intro!: card_insert_le_m1)
   qed auto
-  ultimately have 
+  ultimately have
     f: "finite ({ var_bit_to_var (w, i) | w i. i < n \<and> w \<in> set (Max_Constant.all_variables c) }
     \<union> { operand_bit_to_var (op, i) | op i. i < n \<and> (op = CHR ''a'' \<or> op = CHR ''b'') }
     \<union> { ''carry'' })" and
@@ -381,19 +381,16 @@ proof -
 qed
 
 lemma var_bit_in_IMP_Minus_Minus_variables_then_bit_less_n: "n > 0 \<Longrightarrow> var_bit_to_var (a, b)
-           \<in> set (enumerate_variables (IMP_Minus_To_IMP_Minus_Minus c n)) \<Longrightarrow> b < n" 
+           \<in> set (enumerate_variables (IMP_Minus_To_IMP_Minus_Minus c n)) \<Longrightarrow> b < n"
   apply(frule set_mp[OF IMP_Minus_To_IMP_Minus_Minus_variables])
   by auto
 
 lemma var_bit_in_IMP_Minus_Minus_variables: "v \<in> set (Max_Constant.all_variables c)
   \<Longrightarrow> i < n \<Longrightarrow> var_bit_to_var (v, i) \<in>  set (enumerate_variables (IMP_Minus_To_IMP_Minus_Minus c n))"
   apply(induction c)
-  by(auto simp: assignment_to_binary_def binary_adder_def set_enumerate_variables_seq 
+  by(auto simp: assignment_to_binary_def binary_adder_def set_enumerate_variables_seq
       copy_atom_to_operand_variables adder_def com_list_to_seq_variables full_adder_variables
       binary_subtractor_def subtract_handle_underflow_variables set_enumerate_variables_if
-      var_bit_list_def set_enumerate_variables_while binary_parity_variables
-      binary_right_shift_def assign_shifted_bits_and_zero_most_significant_def
-      assign_shifted_bits_variables
-      split: aexp.splits atomExp.splits)
+      var_bit_list_def set_enumerate_variables_while split: aexp.splits atomExp.splits)
 
 end
