IMP/Com.thy
@@ -1,7 +1,5 @@
 \<^marker>\<open>creator Bilel Ghorbel, Florian Kessler\<close>
-
 section "IMP- A reduced imperative language"
-
 theory Com
   imports
     Main
@@ -14,19 +12,18 @@ begin
 paragraph "Summary"
 text\<open>Syntax definition for IMP-. Based on the syntax definition of IMP\<close>
 
-datatype
-  com = SKIP
-      | Assign vname aexp
-      | Seq    com  com
-      | If     vname com com
-      | While  vname com
+datatype com = SKIP
+  | Assign vname aexp
+  | Seq    com  com
+  | If     vname com com
+  | While  vname com
 
 open_bundle com_syntax
 begin
-notation Assign ("_ ::= _" [1000, 61] 61) and
-         Seq ("_;;/ _"  [60, 61] 60) and
-         If ("(IF _/\<noteq>0 THEN _/ ELSE _)"  [0, 0, 61] 61) and
-         While ("(WHILE _/\<noteq>0 DO _)"  [0, 61] 61)
+notation Assign ("_ ::= _" [1000, 61] 61)
+and Seq ("_;;/ _"  [60, 61] 60)
+and If ("(IF _/\<noteq>0 THEN _/ ELSE _)"  [0, 0, 61] 61)
+and While ("(WHILE _/\<noteq>0 DO _)"  [0, 61] 61)
 end
 
 instantiation com :: order_bot
